Add elaborator into directly `ICom`
This calls the object-level transform functions,
and then reduces the result for easier subsequent proofs

SSA/Projects/InstCombine/Test.lean
@@ -1,5 +1,6 @@
 import SSA.Projects.MLIRSyntax.EDSL
 import SSA.Projects.InstCombine.LLVM.Transform
+import SSA.Projects.InstCombine.LLVM.EDSL
 open MLIR AST
 
 def add_mask := [mlir_op| 
@@ -117,3 +118,17 @@ def comDen : (Option $ Bitvec 32) → (Option $ Bitvec 32) :=
       )
 
 #eval comDen (some <| Bitvec.ofInt 32 (-1))
+
+
+def bb0Icom := [mlir_icom| 
+{
+  ^bb0(%arg0: i32): 
+    %0 = "llvm.mlir.constant"() {value = 8 : i32} : () -> i32
+    %1 = "llvm.mlir.constant"() {value = 31 : i32} : () -> i32
+    %2 = "llvm.ashr"(%arg0, %1) : (i32, i32) -> i32
+    %3 = "llvm.and"(%2, %0) : (i32, i32) -> i32
+    %4 = "llvm.add"(%3, %2) : (i32, i32) -> i32
+    "llvm.return"(%4) : (i32) -> ()
+  }]
+
+example : bb0Icom = com := by rfl
