SSA/Projects/InstCombine/LLVM/EDSL.lean
@@ -1,0 +1,19 @@
+
+import Qq
+import SSA.Projects.MLIRSyntax.EDSL
+import SSA.Projects.InstCombine.LLVM.Transform
+
+open Qq
+open Lean Meta Elab Term
+
+open MLIR.AST in
+elab "[mlir_icom| " reg:mlir_region "]" : term => do
+  let ast_stx ← `([mlir_region| $reg])
+  let ast ← elabTermEnsuringTypeQ ast_stx q(Region)
+  let h_stx ← `(by rfl)
+  let h_isSome ← elabTermEnsuringTypeQ h_stx q(mkCom $ast |>.toOption.isSome)
+  let com := q(mkCom $ast |>.toOption.get $h_isSome)
+  Term.synthesizeSyntheticMVarsNoPostponing
+  withTheReader Core.Context (fun ctx => { ctx with options := ctx.options.setBool `smartUnfolding false }) do
+    withTransparency (mode := TransparencyMode.all) <| 
+      reduce com
